define PCMExt

concurrency/framework/PCM.s.dfy
@@ -9,7 +9,7 @@ abstract module PCM {
 
   type M(==, !new)
 
-  type Ref {
+  type Token {
     function {:extern} loc() : Loc
     function {:extern} get() : M
   }
@@ -46,6 +46,10 @@ abstract module PCM {
 
   predicate transition(a: M, b: M)
 
+  least predicate reachable(a: M, b: M) {
+    a == b || (exists z :: reachable(a, z) && transition(z, b))
+  }
+
   lemma transition_is_monotonic(a: M, b: M, c: M)
   requires transition(a, b)
   requires dot_defined(a, c)
@@ -57,10 +61,10 @@ abstract module PCM {
    */
 
   function method {:extern} transition_update(
-      gshared s: Ref,
-      glinear b: Ref,
+      gshared s: Token,
+      glinear b: Token,
       ghost expected_out: M)
-    : (glinear c: Ref)
+    : (glinear c: Token)
   requires s.loc() == b.loc()
   requires dot_defined(s.get(), b.get()) ==>
     dot_defined(s.get(), expected_out)
@@ -70,44 +74,44 @@ abstract module PCM {
   ensures c.get() == expected_out
   ensures c.loc() == s.loc()
 
-  function method {:extern} get_unit(loc: Loc) : (glinear u: Ref)
+  function method {:extern} get_unit(loc: Loc) : (glinear u: Token)
   ensures u.get() == unit() && u.loc() == loc
 
-  function method {:extern} get_unit_shared(loc: Loc) : (gshared u: Ref)
+  function method {:extern} get_unit_shared(loc: Loc) : (gshared u: Token)
   ensures u.get() == unit() && u.loc() == loc
 
   // This MUST be 'method', as it wouldn't be safe to call this and
   // obtain the postconditions from only ghost 'a' and 'b'.
-  glinear method {:extern} join(glinear a: Ref, glinear b: Ref)
-  returns (glinear sum: Ref)
+  glinear method {:extern} join(glinear a: Token, glinear b: Token)
+  returns (glinear sum: Token)
   requires a.loc() == b.loc()
   ensures dot_defined(a.get(), b.get()) // yes, this is an 'ensures'
   ensures sum.get() == dot(a.get(), b.get())
   ensures sum.loc() == a.loc()
 
   // Same as above: must be 'method', not 'function method'
-  glinear method {:extern} is_valid(gshared a: Ref, glinear b: Ref)
+  glinear method {:extern} is_valid(gshared a: Token, glinear b: Token)
   requires a.loc() == b.loc()
   ensures dot_defined(a.get(), b.get())
 
   // The only reason this is a 'method' and not a 'function method'
   // is so it can easily have two return args.
-  glinear method {:extern} split(glinear sum: Ref, ghost a: M, ghost b: M)
-  returns (glinear a': Ref, glinear b': Ref)
+  glinear method {:extern} split(glinear sum: Token, ghost a: M, ghost b: M)
+  returns (glinear a': Token, glinear b': Token)
   requires dot_defined(a, b)
   requires sum.get() == dot(a, b)
   ensures a'.get() == a && a'.loc() == sum.loc()
   ensures b'.get() == b && b'.loc() == sum.loc()
 
-  function method {:extern} join_shared(gshared s: Ref, gshared t: Ref, ghost expected_q: M)
-    : (gshared q: Ref)
+  function method {:extern} join_shared(gshared s: Token, gshared t: Token, ghost expected_q: M)
+    : (gshared q: Token)
   requires forall r :: le(s.get(), r) && le(t.get(), r) ==> le(expected_q, r)
   requires s.loc() == t.loc()
   ensures q.get() == expected_q
   ensures q.loc() == s.loc()
 
-  function method {:extern} sub(gshared s: Ref, ghost t: M)
-   : (glinear t': Ref)
+  function method {:extern} sub(gshared s: Token, ghost t: M)
+   : (glinear t': Token)
   requires le(t, s.get())
   ensures t'.get() == t
   ensures t'.loc() == s.loc()
